SVAuth/SVX2_Test_Secret.cs
@@ -1,0 +1,134 @@
+﻿using System;
+using System.Collections.Generic;
+using System.Diagnostics.Contracts;
+using System.Linq;
+using System.Threading.Tasks;
+using SVX2;
+
+namespace SVAuth
+{
+    public static class SVX2_Test_Secret
+    {
+        static readonly Principal idpPrincipal = Principal.Of("IdP");
+        static readonly Principal rpPrincipal = Principal.Of("RP");
+
+        static Principal IdPUserPrincipal(string username)
+        {
+            return Principal.Of("IdP:" + username);
+        }
+
+        class SSOSecretParams
+        {
+            // Corresponds to IdPUserPrincipal(username)
+            internal string username;
+        }
+        class SSOSecretGenerator : SecretGenerator/*<SSOSecretParams>*/
+        {
+            protected override PrincipalHandle[] GetReaders(object/*SSOSecretParams*/ theParams)
+            {
+                return new Principal[] { idpPrincipal, rpPrincipal, IdPUserPrincipal(((SSOSecretParams)theParams).username),
+                    // Uncomment to see the verification fail.
+                    //Principal.Of("other")
+                };
+            }
+
+            protected override string RawGenerate(object/*SSOSecretParams*/ theParams)
+            {
+                return "sso:(" + ((SSOSecretParams)theParams).username + ")";
+            }
+
+            protected override bool RawVerify(object/*SSOSecretParams*/ theParams, string secretValue)
+            {
+                return RawGenerate(theParams) == secretValue;
+            }
+        }
+
+        public class SignInIdPReq : SVX_MSG
+        {
+            public string username;
+            // I wonder if we can model the password as an SVX secret too.
+            // Maybe, but it's not the point of using SVX.
+            public string password;
+        }
+        public class SignInRPReq : SVX_MSG
+        {
+            public string username;
+            public Secret ssoSecret;
+        }
+        public class AuthenticationConclusion : SVX_MSG
+        {
+            public PrincipalHandle authenticatedClient;
+            public string idpUsername;
+        }
+
+        public class IdP : Participant
+        {
+            public Principal SVXPrincipal => idpPrincipal;
+            private SSOSecretGenerator ssoSecretGenerator = new SSOSecretGenerator();
+
+            public SignInRPReq SignInIdP(SignInIdPReq req)
+            {
+                if (req.password != "password:" + req.username)
+                    throw new ArgumentException();
+                var userPrincipal = IdPUserPrincipal(req.username);
+                // If this line is commented out, the check for whether it's OK
+                // to send the secret to the client should fail, but that check
+                // isn't implemented yet.
+                VProgram_API.AssumeActsFor(req.sender, userPrincipal);
+                var ssoSecretParams = new SSOSecretParams { username = req.username };
+                var resp = new SignInRPReq {
+                    username = req.username,
+                    ssoSecret = ssoSecretGenerator.Generate(ssoSecretParams)
+                };
+                VProgram_API.Assert(ssoSecretGenerator.Verify(ssoSecretParams, resp.ssoSecret));
+                return resp;
+            }
+        }
+        public class RP : Participant
+        {
+            public Principal SVXPrincipal => rpPrincipal;
+
+            public AuthenticationConclusion SignInRP(SignInRPReq req)
+            {
+                return new AuthenticationConclusion {
+                    authenticatedClient = req.sender,
+                    idpUsername = req.username
+                };
+            }
+        }
+
+        public static bool LoginSafety(AuthenticationConclusion conc) {
+            // BCT accepts this code but silently mistranslates it!
+            //return VProgram_API.ActsForAny(conc.authenticatedClient,
+            //    new PrincipalHandle[] { idpPrincipal, rpPrincipal, IdPUserPrincipal(conc.idpUsername) });
+            var targets = new PrincipalHandle[3];
+            targets[0] = idpPrincipal;
+            targets[1] = rpPrincipal;
+            targets[2] = IdPUserPrincipal(conc.idpUsername);
+            return VProgram_API.ActsForAny(conc.authenticatedClient, targets);
+        }
+
+        [BCTOmitImplementation]
+        public static void Test()
+        {
+            var idp = new IdP();
+            var rp = new RP();
+
+            var aliceIdP = PrincipalFacet.GenerateNew(idpPrincipal);
+            var aliceRP = PrincipalFacet.GenerateNew(rpPrincipal);
+
+            var idpReq = new SignInIdPReq {
+                username = "alice",
+                password = "password:alice",
+                sender = aliceIdP
+            };
+            var rpReq = SVX_Ops.Call(idp.SignInIdP, idpReq);
+
+            // Imagine the SignInRPReq was signed by the IdP.
+            SVX_Ops.Transfer(rpReq, idpPrincipal, aliceRP);
+
+            var conc = SVX_Ops.Call(rp.SignInRP, rpReq);
+            SVX_Ops.Certify(conc, LoginSafety, new Principal[] { idpPrincipal, rpPrincipal });
+        }
+    }
+}
