SVX_Ops/SVX2/FieldFinder.cs
@@ -1,0 +1,68 @@
+﻿using System;
+using System.Collections.Generic;
+using System.Linq;
+using System.Reflection;
+using System.Threading.Tasks;
+
+namespace SVX2
+{
+    // The interface of this class may change as our needs change...
+    static class FieldFinder<TNeedle>
+    {
+        private static HashSet<Type> leafTypes = new HashSet<Type> { typeof(string) };
+
+        internal class Accessor
+        {
+            // XXX readonly?
+            internal string name;
+            // I tried adding a type parameter for the message type, but all
+            // current callers have only a Type anyway, so it wasn't worth it.
+            // ~ t-mattmc@microsoft.com 2016-07-08
+            internal Func<object, TNeedle> getter;
+            internal Action<object, TNeedle> setter;
+        }
+
+        private static IEnumerable<Accessor> FindFieldsImpl(Type messageType)
+        {
+            foreach (var fieldInfo in messageType.GetFields(BindingFlags.Instance | BindingFlags.Public))
+            {
+                Type fieldType = fieldInfo.FieldType;
+                if (typeof(TNeedle).IsAssignableFrom(fieldType))
+                    yield return new Accessor
+                    {
+                        name = fieldInfo.Name,
+                        getter = (msg) => (TNeedle)fieldInfo.GetValue(msg),
+                        setter = (msg, value) => fieldInfo.SetValue(msg, value)
+                    };
+                else if (fieldType.GetTypeInfo().IsPrimitive || fieldType.IsArray || leafTypes.Contains(fieldType))
+                {
+                    // Don't look inside.
+                }
+                else
+                {
+                    // For now, we look inside everything else.
+                    foreach (var nestedFieldAccessor in FindFields(fieldType))
+                        yield return new Accessor
+                        {
+                            name = fieldInfo.Name + "." + nestedFieldAccessor.name,
+                            getter = (msg) => nestedFieldAccessor.getter(fieldInfo.GetValue(msg)),
+                            setter = (msg, value) => nestedFieldAccessor.setter(fieldInfo.GetValue(msg), value),
+                        };
+                }
+            }
+        }
+
+        static Dictionary<Type, IList<Accessor>> cache = new Dictionary<Type, IList<Accessor>>();
+
+        internal static IEnumerable<Accessor> FindFields(Type messageType)
+        {
+            IList<Accessor> ret;
+            if (!cache.TryGetValue(messageType, out ret))
+            {
+                ret = FindFieldsImpl(messageType).ToList().AsReadOnly();
+                cache.Add(messageType, ret);
+            }
+            return ret;
+        }
+    }
+}
