SVX_Ops/SVX2/SymT.cs
@@ -5,27 +5,45 @@ using System.Threading.Tasks;
 
 namespace SVX2
 {
+    class ParticipantId
+    {
+        internal Principal principal;
+        internal string typeFullName;
+
+        public override bool Equals(object other)
+        {
+            var other2 = other as ParticipantId;
+            return other2 != null && principal == other2.principal && typeFullName == other2.typeFullName;
+        }
+
+        public override int GetHashCode()
+        {
+            return Hasher.Start.With(principal.GetHashCode()).With(typeFullName.GetHashCode());
+        }
+    }
     abstract class SymT
     {
         // TODO
-        internal abstract string TypeFullName { get; }
+        internal abstract string MessageTypeFullName { get; }
+        internal abstract IEnumerable<SymT> EmbeddedSymTs { get; }
     }
     class SymTNondet : SymT
     {
-        internal string typeFullName;
+        internal string messageTypeFullName;
 
-        internal override string TypeFullName => typeFullName;
+        internal override string MessageTypeFullName => messageTypeFullName;
+        internal override IEnumerable<SymT> EmbeddedSymTs => new SymT[] { };
     }
     class SymTMethod : SymT
     {
-        internal Principal principal;
-        internal string runtimeTypeFullName;
+        internal ParticipantId participantId;
         internal string methodName;
         internal string methodReturnTypeFullName;
         internal string[] methodArgTypeFullNames;
         internal SymT[] inputSymTs;
 
-        internal override string TypeFullName => methodReturnTypeFullName;
+        internal override string MessageTypeFullName => methodReturnTypeFullName;
+        internal override IEnumerable<SymT> EmbeddedSymTs => inputSymTs;
     }
     class SymTTransfer : SymT
     {
@@ -34,8 +52,10 @@ namespace SVX2
         // principals and no facets, so avoid a cast in the emit.
         internal Principal producer, sender;
 
-        internal override string TypeFullName => originalSymT.TypeFullName;
+        internal override string MessageTypeFullName => originalSymT.MessageTypeFullName;
+        internal override IEnumerable<SymT> EmbeddedSymTs => new SymT[] { originalSymT };
     }
+#if false
     class NestedSymTEntry
     {
         internal string fieldPath;  // dotted
@@ -46,14 +66,16 @@ namespace SVX2
         internal SymT rootSymT;
         internal List<NestedSymTEntry> nestedSymTs;
 
-        internal override string TypeFullName => rootSymT.TypeFullName;
+        internal override string MessageTypeFullName => rootSymT.MessageTypeFullName;
     }
+#endif
     class CertificationRequest
     {
         internal SymT scrutineeSymT;
         internal string methodDeclaringTypeFullName;
         internal string methodName;
         internal string methodArgTypeFullName;
+        internal ParticipantId[] predicateParticipants;
         internal Principal[] trustedParties;
     }
 
