SVX_Ops/SVX2/VProgramEmitter.cs
@@ -22,14 +22,25 @@ namespace SVX2
             Contract.Assume(Regex.IsMatch(x, "^[_A-Za-z0-9]*$"));
             return "\"" + x + "\"";
         }
+        string EmitPrincipal(Principal p) => "SVX2.Principal.Of(" + Quote(p.name) + ")";
         string EmitPrincipalOrNondet(Principal p)
+            => (p == null) ? "SVX2.VProgram_API.Nondet<SVX2.Principal>()" : EmitPrincipal(p);
+
+        // Nested types... Should we use a wrapper class in SymTs (that is
+        // still serializable, unlike System.Type) and move this method there?
+        string FormatTypeFullName(string fullName) => fullName.Replace('+', '.');
+
+        HashSet<ParticipantId> participantsSeen = new HashSet<ParticipantId>();
+        void ScanParticipants(SymT symT)
         {
-            if (p == null)
-                return "SVX2.VProgram_API.Nondet<SVX2.Principal>()";
-            else
-                return "SVX2.Principal.Of(" + Quote(p.name) + ")";
+            var symTMethod = symT as SymTMethod;
+            if (symTMethod != null)
+                participantsSeen.Add(symTMethod.participantId);
+            foreach (var embedded in symT.EmbeddedSymTs)
+                ScanParticipants(embedded);
         }
-        string Visit(SymT symT)
+
+        string EmitMessage(SymT symT)
         {
             // XXX: Currently we cannot deal with non-public participant classes
             // and methods.  It's an open question if we should be able to and
@@ -46,16 +57,18 @@ namespace SVX2
             if ((symTNondet = symT as SymTNondet) != null)
             {
                 outputVarName = nextVar("msg");
-                sb.AppendFormat("{0} {1} = SVX2.VProgram_API.Nondet<{0}>();\n", symTNondet.typeFullName, outputVarName);
+                sb.AppendFormat("{0} {1} = SVX2.VProgram_API.Nondet<{0}>();\n",
+                    FormatTypeFullName(symTNondet.messageTypeFullName), outputVarName);
             }
             else if ((symTMethod = symT as SymTMethod) != null)
             {
                 // This has side effects, so evaluate it right away.
-                string[] argVarNames = (from i in symTMethod.inputSymTs select Visit(i)).ToArray();
+                string[] argVarNames = (from i in symTMethod.inputSymTs select EmitMessage(i)).ToArray();
                 outputVarName = nextVar("msg");
                 sb.AppendFormat("{0} {1} = SVX2.VProgram_API.GetParticipant<{2}>(SVX2.Principal.Of({3})).{4}({5});\n",
-                    symTMethod.methodReturnTypeFullName, outputVarName,
-                    symTMethod.runtimeTypeFullName, Quote(symTMethod.principal.name), symTMethod.methodName,
+                    FormatTypeFullName(symTMethod.methodReturnTypeFullName), outputVarName,
+                    FormatTypeFullName(symTMethod.participantId.typeFullName),
+                    Quote(symTMethod.participantId.principal.name), symTMethod.methodName,
                     string.Join(", ", argVarNames));
             }
             // This needs a rewrite to avoid depending on Equals.
@@ -77,16 +90,32 @@ namespace SVX2
                 string producerVarName = nextVar("producer");
                 sb.AppendFormat("SVX2.PrincipalHandle {0} = {1};\n", producerVarName, EmitPrincipalOrNondet(symTTransfer.producer));
                 outputVarName = nextVar("msg");
-                sb.AppendFormat("{0} {1};\n", symTTransfer.TypeFullName, outputVarName);
+                sb.AppendFormat("{0} {1};\n", FormatTypeFullName(symTTransfer.MessageTypeFullName), outputVarName);
                 sb.AppendFormat("if (SVX2.VProgram_API.ActsForAny({0}, trustedParties)) {{\n", producerVarName);
                 {
-                    string inputVarName = Visit(symTTransfer.originalSymT);
+                    string inputVarName = EmitMessage(symTTransfer.originalSymT);
                     sb.AppendFormat("{0} = {1};\n", outputVarName, inputVarName);
                 }
-                sb.AppendFormat("}} else {0} = SVX2.VProgram_API.Nondet<{1}>();\n", outputVarName, symTTransfer.TypeFullName);
+                sb.AppendFormat("}} else {0} = SVX2.VProgram_API.Nondet<{1}>();\n",
+                    outputVarName, FormatTypeFullName(symTTransfer.MessageTypeFullName));
                 sb.AppendFormat("{0}.producer = {1};\n", outputVarName, producerVarName);
                 sb.AppendFormat("{0}.sender = {1};\n", outputVarName, EmitPrincipalOrNondet(symTTransfer.sender));
-                // TODO: Add Borne assumptions for secrets
+
+                /* Currently, we assume all concrete message types are in the
+                 * SVAuth assembly.  To lift that restriction, we'd have to
+                 * either include the assembly qualified name in the SymT or
+                 * just look for the type in all uploaded assemblies.  Once we
+                 * can have N parties with assemblies named "SVAuth" with
+                 * different code or even different definitions of the
+                 * transferred message types (!), we'll need to add the hash of
+                 * the assembly and we'll need to copy messages one field at a
+                 * time between the differently defined types. */
+                Type messageType = Type.GetType(symTTransfer.MessageTypeFullName + ", SVAuth");
+                foreach (var acc in FieldFinder<Secret>.FindFields(messageType))
+                {
+                    sb.AppendFormat("SVX2.VProgram_API.AssumeBorne({0}.producer, {0}.{1}.secretValue);\n", outputVarName, acc.name);
+                    sb.AppendFormat("SVX2.VProgram_API.AssumeBorne({0}.sender, {0}.{1}.secretValue);\n", outputVarName, acc.name);
+                }
             }
             else
             {
@@ -107,12 +136,18 @@ namespace SVX2
             for (int i = 0; i < certReq.trustedParties.Length; i++)
                 sb.AppendFormat("trustedParties[{0}] = {1};\n", i, EmitPrincipalOrNondet(certReq.trustedParties[i]));
 
-            string scrutineeVarName = Visit(certReq.scrutineeSymT);
+            participantsSeen.UnionWith(certReq.predicateParticipants);
+            ScanParticipants(certReq.scrutineeSymT);
+            foreach (var participant in participantsSeen)
+                sb.AppendFormat("SVX2.VProgram_API.CreateParticipant({0}, new {1}());\n",
+                    EmitPrincipal(participant.principal), FormatTypeFullName(participant.typeFullName));
+
+            string scrutineeVarName = EmitMessage(certReq.scrutineeSymT);
             // We list System.Diagnostics.Contracts as a direct dependency as a
             // good practice, even though we'll nearly always get it as an
             // indirect dependency.
             sb.AppendFormat("System.Diagnostics.Contracts.Contract.Assert({0}.{1}({2}));\n",
-                certReq.methodDeclaringTypeFullName, certReq.methodName, scrutineeVarName);
+                FormatTypeFullName(certReq.methodDeclaringTypeFullName), certReq.methodName, scrutineeVarName);
             sb.Append("}\n");
             sb.Append("}\n");
         }
